src/Refinement.v
@@ -96,12 +96,18 @@ Section refinement.
     f_simpl. rewrite <- (f_subst_initials_final_formula pre w)...
     rewrite <- simpl_subst_initials_and. unfold subst_initials.
     rewrite <- f_foralllist_one_point... rewrite (f_foralllist_elim_binders (as_var <$> w)).
-    rewrite f_impl_dup_hyp.
-    erewrite eqlist_rewrite_l at 2. Unshelve.
-    3: { rewrite <- list_fmap_compose. reflexivity. }
-    rewrite f_and_assoc. rewrite H0. rewrite f_impl_elim. rewrite f_foralllist_one_point...
-    rewrite fold_subst_initials. rewrite f_subst_initials_final_formula... reflexivity.
+    rewrite f_impl_dup_hyp. rewrite f_and_assoc. rewrite H0. rewrite f_impl_elim.
+    rewrite f_foralllist_one_point... rewrite fold_subst_initials.
+    rewrite f_subst_initials_final_formula... reflexivity.
   Qed.
+
+  (* Lemma r_seq w pre mid post `{FormulaFinal _ pre} `{FormulaFinal _ mid} : *)
+  (*   <{ *w : [pre, post] }> ⊑ <{ *w : [pre, mid]; *w : [mid, post] }>. *)
+  (* Proof with auto. *)
+  (*   intros A Hfinal. simpl. f_simpl. unfold subst_initials. *)
+  (*   rewrite <- f_foralllist_one_point at 1... *)
+  (*   rewrite <- f_foralllist_one_point at 1... *)
+  (*   f_equiv. f_equiv. rewrite fold_subst_initials. *)
 
   Lemma r_assignment w xs pre post ts `{FormulaFinal _ pre} `{OfSameLength _ _ xs ts} :
     length xs ≠ 0 →
@@ -110,7 +116,7 @@ Section refinement.
     <{ *w, *xs : [pre, post] }> ⊑ <{ *xs := *$(FinalRhsTerm <$> ts)  }>.
   Proof with auto.
     intros Hlength Hnodup proviso A Hfinal. simpl. rewrite wp_asgn.
-    rewrite <- (f_subst_initials_final_formula pre w)...
+    rewrite <- (f_subst_initials_final_formula pre (w ++ xs))...
     rewrite <- simpl_subst_initials_and. rewrite fmap_app.
     unfold subst_initials. rewrite <- f_foralllist_one_point...
     rewrite f_foralllist_app. rewrite (f_foralllist_elim_binders (as_var <$> w)).
@@ -118,16 +124,18 @@ Section refinement.
     2:{ rewrite length_fmap... }
     2:{ apply NoDup_fmap... apply as_var_inj. }
     erewrite eqlist_rewrite. Unshelve.
-    4: { do 2 rewrite fmap_app. do 2 rewrite <- list_fmap_compose. reflexivity. }
-    3: { rewrite fmap_app. reflexivity. }
+    4: { do 2 rewrite fmap_app. reflexivity. }
+    3: { do 2 rewrite fmap_app. reflexivity. }
     rewrite f_eqlist_app. rewrite f_impl_dup_hyp. rewrite (f_and_assoc _ pre).
     rewrite f_and_assoc in proviso. rewrite proviso. clear proviso. rewrite simpl_ssubst_impl.
     f_simpl. rewrite <- f_eqlist_app.
     erewrite eqlist_rewrite. Unshelve.
-    4: { rewrite <- fmap_app. rewrite list_fmap_compose. reflexivity. }
-    3: { rewrite <- fmap_app. reflexivity. }
+    4: { do 2 rewrite <- list_fmap_compose. rewrite <- fmap_app. rewrite list_fmap_compose.
+         reflexivity. }
+    3: { do 2 rewrite <- list_fmap_compose. rewrite <- fmap_app. rewrite list_fmap_compose.
+         reflexivity. }
     pose proof (@f_foralllist_one_point M
-                  (initial_var_of <$> (w ++ xs)) ((TVar ∘ as_var <$> (w++xs)))) as ->...
+                  (initial_var_of <$> (w ++ xs)) ((TVar <$> (as_var <$> (w++xs))))) as ->...
     rewrite fold_subst_initials. rewrite f_subst_initials_final_formula.
     2: { unfold formula_final. intros. apply fvars_ssubst_superset in H1.
          set_unfold. destruct H1.
